code/k256/Hacl.Impl.K256.PointAdd.fst
@@ -1,0 +1,27 @@
+module Hacl.Impl.K256.PointAdd
+
+open FStar.HyperStack
+open FStar.HyperStack.ST
+open FStar.Mul
+
+open Lib.IntTypes
+open Lib.Buffer
+
+module ST = FStar.HyperStack.ST
+module LSeq = Lib.Sequence
+module BSeq = Lib.ByteSequence
+module S = Spec.K256
+
+open Hacl.K256.Field
+open Hacl.Impl.K256.Point
+
+#set-options "--z3rlimit 50 --fuel 0 --ifuel 0"
+
+
+val point_add (out p q:point) : Stack unit
+  (requires fun h ->
+    live h out /\ live h p /\ live h q /\
+    eq_or_disjoint out p /\ eq_or_disjoint out q /\ eq_or_disjoint p q /\
+    point_inv h p /\ point_inv h q)
+  (ensures fun h0 _ h1 -> modifies (loc out) h0 h1 /\ point_inv h1 out /\
+    point_as_nat3_proj h1 out == S.point_add (point_as_nat3_proj h0 p) (point_as_nat3_proj h0 q))
