code/k256/Hacl.K256.Field.fsti
@@ -1,0 +1,155 @@
+module Hacl.K256.Field
+
+open FStar.HyperStack
+open FStar.HyperStack.ST
+open FStar.Mul
+
+open Lib.IntTypes
+open Lib.Buffer
+
+module ST = FStar.HyperStack.ST
+module LSeq = Lib.Sequence
+module BSeq = Lib.ByteSequence
+module S = Spec.K256
+
+module BD = Hacl.Bignum.Definitions
+
+
+#set-options "--z3rlimit 50 --fuel 0 --ifuel 0"
+
+(**
+  This is a naive implementation of field arithmetic for testing purposes
+*)
+
+inline_for_extraction noextract
+let felem = lbuffer uint64 4ul
+
+noextract
+let as_nat (h:mem) (e:felem) : GTot nat = BD.bn_v #U64 #4ul h e
+
+noextract
+let feval (h:mem) (e:felem) : GTot S.elem = as_nat h e % S.prime
+
+noextract
+let fe_lt_prime (h:mem) (e:felem) = as_nat h e < S.prime
+
+
+inline_for_extraction noextract
+val create_felem: unit -> StackInline felem
+  (requires fun h -> True)
+  (ensures  fun h0 f h1 ->
+    stack_allocated f h0 h1 (LSeq.create 4 (u64 0)) /\
+    as_nat h1 f == 0)
+
+
+val load_felem: f:felem -> b:lbuffer uint8 32ul -> Stack unit
+  (requires fun h ->
+    live h f /\ live h b /\ disjoint f b /\
+    BSeq.nat_from_bytes_be (as_seq h b) < S.prime)
+  (ensures  fun h0 _ h1 -> modifies (loc f) h0 h1 /\
+    as_nat h1 f == BSeq.nat_from_bytes_be (as_seq h0 b))
+
+
+val store_felem: b:lbuffer uint8 32ul -> f:felem -> Stack unit
+  (requires fun h ->
+    live h b /\ live h f /\ disjoint f b /\
+    fe_lt_prime h f)
+  (ensures  fun h0 _ h1 -> modifies (loc b) h0 h1 /\
+    as_seq h1 b == BSeq.nat_to_bytes_be 32 (as_nat h0 f))
+
+
+inline_for_extraction noextract
+val set_zero: f:felem -> Stack unit
+  (requires fun h -> live h f)
+  (ensures  fun h0 _ h1 -> modifies (loc f) h0 h1 /\
+    as_nat h1 f == 0)
+
+
+inline_for_extraction noextract
+val set_one: f:felem -> Stack unit
+  (requires fun h -> live h f)
+  (ensures  fun h0 _ h1 -> modifies (loc f) h0 h1 /\
+    as_nat h1 f == 1)
+
+
+inline_for_extraction noextract
+val copy_felem (f1 f2:felem) : Stack unit
+  (requires fun h ->
+    live h f1 /\ live h f2 /\ disjoint f1 f2)
+  (ensures  fun h0 _ h1 -> modifies (loc f1) h0 h1 /\
+    as_seq h1 f1 == as_seq h0 f2)
+
+
+val times_3b (out f:felem) : Stack unit
+  (requires fun h ->
+    live h f /\ live h out /\ eq_or_disjoint out f /\
+    fe_lt_prime h f)
+  (ensures  fun h0 _ h1 -> modifies (loc out) h0 h1 /\
+    as_nat h1 out = S.fmul (S.fmul 3 S.b) (as_nat h0 f) /\
+    fe_lt_prime h1 out)
+
+
+val times_24b (out f:felem) : Stack unit
+  (requires fun h ->
+    live h f /\ live h out /\ eq_or_disjoint out f /\
+    fe_lt_prime h f)
+  (ensures  fun h0 _ h1 -> modifies (loc out) h0 h1 /\
+    as_nat h1 out = S.fmul (S.fmul 24 S.b) (as_nat h0 f) /\
+    fe_lt_prime h1 out)
+
+
+val times_small_num (out f:felem) (num:uint64) : Stack unit
+  (requires fun h -> v num <= 8 /\ // a maximum value for point addition and doubling
+    live h f /\ live h out /\ eq_or_disjoint out f /\
+    fe_lt_prime h f)
+  (ensures  fun h0 _ h1 -> modifies (loc out) h0 h1 /\
+    as_nat h1 out = S.fmul (v num) (as_nat h0 f) /\
+    fe_lt_prime h1 out)
+
+
+val fadd (out f1 f2: felem) : Stack unit
+  (requires fun h ->
+    live h out /\ live h f1 /\ live h f2 /\
+    eq_or_disjoint out f1 /\ eq_or_disjoint out f2 /\ eq_or_disjoint f1 f2 /\
+    fe_lt_prime h f1 /\ fe_lt_prime h f2)
+  (ensures  fun h0 _ h1 -> modifies (loc out) h0 h1 /\
+    as_nat h1 out == S.fadd (as_nat h0 f1) (as_nat h0 f2) /\
+    fe_lt_prime h1 out)
+
+
+val fsub (out f1 f2: felem) : Stack unit
+  (requires fun h ->
+    live h out /\ live h f1 /\ live h f2 /\
+    eq_or_disjoint out f1 /\ eq_or_disjoint out f2 /\ eq_or_disjoint f1 f2 /\
+    fe_lt_prime h f1 /\ fe_lt_prime h f2)
+  (ensures  fun h0 _ h1 -> modifies (loc out) h0 h1 /\
+    as_nat h1 out == S.fsub (as_nat h0 f1) (as_nat h0 f2) /\
+    fe_lt_prime h1 out)
+
+
+val fmul (out f1 f2: felem) : Stack unit
+  (requires fun h ->
+    live h out /\ live h f1 /\ live h f2 /\
+    eq_or_disjoint out f1 /\ eq_or_disjoint out f2 /\ eq_or_disjoint f1 f2 /\
+    fe_lt_prime h f1 /\ fe_lt_prime h f2)
+  (ensures  fun h0 _ h1 -> modifies (loc out) h0 h1 /\
+    as_nat h1 out == S.fmul (as_nat h0 f1) (as_nat h0 f2) /\
+    fe_lt_prime h1 out)
+
+
+val fsqr (out f: felem) : Stack unit
+  (requires fun h ->
+    live h out /\ live h f /\ eq_or_disjoint out f /\
+    fe_lt_prime h f)
+  (ensures  fun h0 _ h1 -> modifies (loc out) h0 h1 /\
+    as_nat h1 out == S.fmul (as_nat h0 f) (as_nat h0 f) /\
+    fe_lt_prime h1 out)
+
+
+val finv (out f: felem) : Stack unit
+  (requires fun h ->
+    live h out /\ live h f /\ eq_or_disjoint out f /\
+    fe_lt_prime h f)
+  (ensures  fun h0 _ h1 -> modifies (loc out) h0 h1 /\
+    as_nat h1 out == S.finv (as_nat h0 f)  /\
+    fe_lt_prime h1 out)
